verified/svcapi.s.dfy
@@ -1,0 +1,102 @@
+include "kom_common.s.dfy"
+include "pagedb.s.dfy"
+include "sha/sha256.s.dfy"
+
+predicate isReturningSvc(s:state)
+    requires ValidState(s) && mode_of_state(s) != User
+{
+    reveal ValidRegState();
+    s.conf.ex.ExSVC? && s.regs[R0] != KOM_SVC_EXIT
+}
+
+// SVCs return up to 9 registers
+type SvcReturnRegs = (word, word, word, word, word, word, word, word, word)
+
+function svcHmacAttest(s:state, d:PageDb, dispPg:PageNr): seq<word>
+    requires validPageDb(d) && validDispatcherPage(d, dispPg)
+    requires ValidState(s) && mode_of_state(s) != User
+    requires isReturningSvc(s)
+{
+    var addrspace := d[dispPg].addrspace;
+    assert validAddrspacePage(d, addrspace) by { reveal_validPageDb(); }
+    var enclave_measurement := SHA256(WordSeqToBytes(d[addrspace].entry.measurement));
+    var user_words := [s.regs[R1], s.regs[R2], s.regs[R3], s.regs[R4],
+        s.regs[R5], s.regs[R6], s.regs[R7], s.regs[R8]];
+
+    // produce an attestation
+    var message := user_words + enclave_measurement + SeqRepeat(8, 0);
+    HMAC_SHA256(AttestKey(), WordSeqToBytes(message))
+}
+
+function svcHmacVerify(s:state, d:PageDb, dispPg:PageNr): seq<word>
+    requires validPageDb(d) && validDispatcherPage(d, dispPg)
+    requires ValidState(s) && mode_of_state(s) != User
+    requires isReturningSvc(s)
+{
+    var addrspace := d[dispPg].addrspace;
+    assert validAddrspacePage(d, addrspace) by { reveal_validPageDb(); }
+
+    // verify an attestation
+    var message := d[dispPg].entry.verify_words + d[dispPg].entry.verify_measurement + SeqRepeat(8, 0);
+    HMAC_SHA256(AttestKey(), WordSeqToBytes(message))
+}
+
+function svcMapData(d:PageDb, asPg:PageNr, page:word, mapping:word) : (PageDb, word)
+    requires validPageDb(d) && validAddrspacePage(d, asPg)
+{
+    // TODO: weaken isValidMappingTarget to permit some mappings outside the InitState
+    var mapErr := isValidMappingTarget(d, asPg, mapping);
+    if !validPageNr(page) || pageIsFree(d, page) || d[page].addrspace != asPg
+        || !d[page].entry.SparePage?
+        then (d, KOM_ERR_INVALID_PAGENO)
+    else if mapErr != KOM_ERR_SUCCESS
+        then (d, mapErr)
+    else
+        // update page to zero-filled data page, and mapping in l2
+        var d1 := d[page := d[page].(entry := DataPage(SeqRepeat(PAGESIZE/WORDSIZE, 0)))];
+        var abs_mapping := wordToMapping(mapping);
+        var l2pte := SecureMapping(page, abs_mapping.perm.w, abs_mapping.perm.x);
+        var d2 := updateL2Pte(d1, asPg, abs_mapping, l2pte);
+        (d2, KOM_ERR_SUCCESS)
+}
+
+function svcHandled(s:state, d:PageDb, dispPg:PageNr): (SvcReturnRegs, PageDb)
+    requires validPageDb(d) && validDispatcherPage(d, dispPg)
+    requires ValidState(s) && mode_of_state(s) != User
+    requires isReturningSvc(s)
+{
+    var addrspace := d[dispPg].addrspace;
+    assert validAddrspacePage(d, addrspace) by { reveal_validPageDb(); }
+    var enclave_measurement := SHA256(WordSeqToBytes(d[addrspace].entry.measurement));
+    var callno := s.regs[R0];
+    var user_words := [s.regs[R1], s.regs[R2], s.regs[R3], s.regs[R4],
+        s.regs[R5], s.regs[R6], s.regs[R7], s.regs[R8]];
+    var success_regs := (KOM_ERR_SUCCESS, 0, 0, 0, 0, 0, 0, 0, 0);
+
+    if callno == KOM_SVC_ATTEST then
+        // produce an attestation
+        var hmac := svcHmacAttest(s, d, dispPg);
+        ((KOM_ERR_SUCCESS, hmac[0], hmac[1], hmac[2], hmac[3], hmac[4], hmac[5],
+            hmac[6], hmac[7]), d)
+    else if callno == KOM_SVC_VERIFY_STEP0 then
+        // stash user-provided words in pagedb for a subsequent STEP1 call
+        // (this is a cheesy workaround to avoid reading enclave memory)
+        var ret_pagedb := d[dispPg := d[dispPg].(entry := d[dispPg].entry.(verify_words := user_words))];
+        (success_regs, ret_pagedb)
+    else if callno == KOM_SVC_VERIFY_STEP1 then
+        // stash user-provided words in pagedb for a subsequent STEP1 call
+        // (this is a cheesy workaround to avoid reading enclave memory)
+        var ret_pagedb := d[dispPg := d[dispPg].(entry := d[dispPg].entry.(verify_measurement := user_words))];
+        (success_regs, ret_pagedb)
+    else if callno == KOM_SVC_VERIFY_STEP2 then
+        // verify the attestation provided by the previous step0 call plus this
+        var hmac := svcHmacVerify(s, d, dispPg);
+        var ok := if user_words == hmac then 1 else 0;
+        (success_regs.(1 := ok), d)
+    else if callno == KOM_SVC_MAP_DATA then
+        var (retDb, retErr) := svcMapData(d, addrspace, s.regs[R1], s.regs[R2]);
+        (success_regs.(0 := retErr), retDb)
+    // TODO: KOM_SVC_INIT_L2PTABLE, KOM_SVC_UNMAP
+    else
+        (success_regs.(0 := KOM_ERR_INVALID), d)
+}
